Minimmit/Analysis/Liveness/Lemma5_6.lean
@@ -22,11 +22,11 @@ theorem correct_leader_finalises (hn : 5 * f + 1 ≤ n) (hinit : Init s₀)
     (hh : Honest f Δ lead s₀ instrs) (hb : ByzBound f s₀ instrs)
     (hs : PartialSync Δ GST s₀ instrs) {v : View} (hv : 1 ≤ v.val) (hi : Correct s₀ instrs (lead v))
     {t : Nat} (hfirst : FirstEntry s₀ instrs v t) (hgst : GST.val ≤ t) :
-    ∃ b : Block Tx, b.view = v
-      ∧ (∃ t', ∀ j, Action.send (.propose (lead v) b) j ∈ (instrs t').actions (lead v))
+    ∃ b : Block n Tx, b.view = v ∧ b.signer = some (lead v)
+      ∧ (∃ t', ∀ j, Action.send (.propose b) j ∈ (instrs t').actions (lead v))
       ∧ ReceivesL f instrs b := by
   obtain ⟨e, R⟩ := leader_round hinit hh hs (le_refl Δ) hv hi hfirst hgst
-  refine ⟨leaderBlockAt f lead s₀ instrs v e, leaderBlockAt_view hinit hh hb hs R,
+  refine ⟨leaderBlockAt f lead s₀ instrs v e, leaderBlockAt_view hinit hh hb hs R, rfl,
     ⟨e, fun j => leader_proposes hinit hh hb hs R j⟩, ?_⟩
   right
   refine (card_correctSet hb).trans (Finset.card_le_card fun r hr => ?_)
